more patching

src/certigrad/aevb/util.lean
@@ -13,7 +13,7 @@ namespace aevb
 structure arch : Type := (bs n_x n_in nz ne nd : ℕ)
 
 structure weights (a : arch) : Type :=
-  (batch_start : ℝ)
+  (batch_num : ℕ)
   (W_encode₁ : T [a^.ne, a^.n_in])
   (W_encode₂ : T [a^.ne, a^.ne])
   (W_encode_μ W_encode_logσ₂ : T [a^.nz, a^.ne])
@@ -23,8 +23,8 @@ structure weights (a : arch) : Type :=
 
 section label
 open certigrad.label
-@[cgsimp] def mk_input_dict : Π {a : arch} (ws : weights a) (g : graph), env
-| a ws g := env.insert_all [(ID.str batch_start, []),
+@[cgsimp] def mk_input_dict : Π {a : arch} (ws : weights a) (x_data : T [a^.n_in, a^.n_x]) (g : graph), env
+| a ws x_data g := env.insert_all [(ID.str x, [a^.n_in, a^.bs]),
                             (ID.str W_encode₁, [a^.ne, a^.n_in]),
                             (ID.str W_encode₂, [a^.ne, a^.ne]),
                             (ID.str W_encode_μ, [a^.nz, a^.ne]),
@@ -32,7 +32,7 @@ open certigrad.label
                             (ID.str W_decode₁, [a^.nd, a^.nz]),
                             (ID.str W_decode₂, [a^.nd, a^.nd]),
                             (ID.str W_decode_p, [a^.n_in, a^.nd])]
-                           ⟦ws^.batch_start, ws^.W_encode₁, ws^.W_encode₂, ws^.W_encode_μ, ws^.W_encode_logσ₂,
+                           ⟦T.get_col_range a^.bs x_data (a^.bs * ws^.batch_num), ws^.W_encode₁, ws^.W_encode₂, ws^.W_encode_μ, ws^.W_encode_logσ₂,
                             ws^.W_decode₁, ws^.W_decode₂, ws^.W_decode_p⟧
 end label
 
