src/certigrad/aevb/transformations.lean
@@ -30,7 +30,7 @@ do whnf_target,
 
 #print "proving integrate_kl_sound..."
 lemma integrate_kl_sound (a : arch) (ws : weights a) (x_data : T [a^.n_in, a^.n_x]) :
-let g₀ : graph := graph_naive a x_data, fdict : env := mk_input_dict ws g₀ in
+let g₀ : graph := graph_naive a x_data, fdict : env := mk_input_dict ws x_data g₀ in
 ∀ (tgt : reference) (idx : ℕ) (H_at_idx : at_idx g₀^.targets idx tgt) (θ : T tgt.2),
 E (graph.to_dist (λ m, ⟦sum_costs m (integrate_kl g₀)^.costs⟧) (env.insert tgt θ fdict) (integrate_kl g₀)^.nodes) dvec.head
 =
@@ -40,7 +40,7 @@ sorry
 
 #print "proving reparam_sound..."
 lemma reparam_sound (a : arch) (ws : weights a) (x_data : T [a^.n_in, a^.n_x]) :
-let g₁ : graph := integrate_kl (graph_naive a x_data), fdict : env := mk_input_dict ws g₁ in
+let g₁ : graph := integrate_kl (graph_naive a x_data), fdict : env := mk_input_dict ws x_data g₁ in
 ∀ (tgt : reference) (idx : ℕ) (H_at_idx : at_idx g₁^.targets idx tgt) (θ : T tgt.2),
 E (graph.to_dist (λ m, ⟦sum_costs m (reparam g₁)^.costs⟧) (env.insert tgt θ fdict) (reparam g₁)^.nodes) dvec.head
 =
@@ -53,7 +53,7 @@ by prove_transformation ```(reparameterize_correct [ID.str label.encoding_loss, 
 #print "proving aevb_transformations_sound..."
 
 lemma aevb_transformations_sound {a : arch} (ws : weights a) (x_data : T [a^.n_in, a^.n_x]) :
-let g₀ : graph := naive_aevb a x_data, g_aevb : graph := reparam (integrate_kl g₀), fdict : env := mk_input_dict ws g₀ in
+let g₀ : graph := naive_aevb a x_data, g_aevb : graph := reparam (integrate_kl g₀), fdict : env := mk_input_dict ws x_data g₀ in
 ∀ (tgt : reference) (idx : ℕ) (H_at_idx : at_idx g₀^.targets idx tgt) (θ : T tgt.2),
 E (graph.to_dist (λ m, ⟦sum_costs m g₀^.costs⟧) (env.insert tgt θ fdict) g₀^.nodes) dvec.head
 =
